assignments/midterm/Midterm.v
@@ -1,0 +1,219 @@
+(** CS6225 Spring 2025: Programs and proofs -- Mid Term *)
+
+(***************************************
+ ** Instructions
+ ***************************************
+
+   This is a take home exam, with 24 hours for the exam. Strictly no late
+   submissions allowed. Submit your solutions through course moodle.
+
+   Completed solutions should not have any [Abort]ed proofs. If there are, they
+   will get [0] points. There are a few lemmas and theorems for which the proof
+   ends with [Admitted]. For example, see [fib_succ_add] and
+   [fib_fib_tail_rec']. Those are the only ones for which you may leave the
+   proof as admitted and use it in the subsequent theorems ([fib_ok] for
+   example). Your solution will not have any other [Admitted] proofs. Any other
+   use of [Admitted] proofs will get [0] points. *)
+
+Require Import Frap MidtermSig.
+
+(***************************************
+ ** Swivel
+ ***************************************)
+
+Inductive tree :=
+  | Leaf
+  | Node (v : nat) (lt rt : tree).
+  
+Fixpoint rightmost (tr: tree) : option nat :=
+  match tr with
+  | Leaf => None
+  | Node v _ rt =>
+    match rt with
+    | Leaf => Some v
+    | _ => rightmost rt
+    end
+  end.
+  
+Fixpoint leftmost (tr : tree) : option nat := None. (* Remove [None] and fill in *)
+(* 3 points *)
+  
+Fixpoint swivel tr :=
+  match tr with
+  | Leaf => Leaf
+  | Node v lt rt => Node v (swivel rt) (swivel lt)
+  end.
+  
+Theorem swivel_ok : forall tr, 
+  leftmost tr = rightmost (swivel tr).
+(* 5 points *)
+Proof.
+Abort.
+
+(***************************************
+ ** Fibonacci Sequence
+ ***************************************)
+
+Fixpoint fib n :=
+  match n with
+  | 0 => 1
+  | S n' => match n' with
+            | 0 => 1
+            | S n'' => fib n'' + fib n'
+            end
+  end.
+
+Fixpoint fib_tail_rec' n a b :=
+  match n with
+  | 0 => a
+  | S n' => fib_tail_rec' n' b (a+b)
+  end.
+
+Definition fib_tail_rec n := n + 0.
+(* Remove [n + 0] and fill in correct definition *)
+(* 2 points *)
+
+Example ex1: fib 10 = 89.
+Proof.
+  auto.
+Qed.
+
+Example ex2: fib_tail_rec 10 = 89.
+Proof.
+  auto.
+Abort.
+
+Lemma fib_succ_add: forall n,
+  fib n + fib (n+1) = fib(n+2).
+(* 5 points *)
+Proof.
+  (* FILL IN *)
+Admitted.
+
+Lemma fib_fib_tail_rec': forall n k,
+  fib_tail_rec' n (fib k) (fib (k+1)) = fib (k+n).
+(* 5 points *)
+Proof.
+  (* FILL IN *)
+Admitted.
+
+Theorem fib_ok : forall n, fib n = fib_tail_rec n.
+(* 5 points *)
+Proof.
+  (* FILL IN *)
+Abort.
+
+(***************************************
+ ** List.rev is involutive
+ **************************************)
+
+Require Import List.
+Import ListNotations.
+
+Theorem rev_involutive : forall (A:Type) (l : list A), rev (rev l) = l.
+(* 5 points *)
+Proof.
+Abort.
+
+(***************************************
+ ** Insertion sort
+ ***************************************
+ 
+ 
+  We will define insertion sort and prove it right. Consider the following 
+  idea. Given the input list l = [4;5;1;3], sorting proceeds like this:
+
+  Using an auxilliary list [sorted]:
+
+  l=[4;5;1;3] aux=[]
+  l=[5;1;3]   aux=[4]
+  l=[1;3]     aux=[4;5]
+  l=[3]       aux=[1;4;5]
+  l=[]        aux=[1;3;4;5]
+  
+  Observe that [aux] is always sorted. The idea is that, at each step, 
+  we take one element from [l] and insert into [aux] at the right position 
+  so that [aux] remains sorted. When [l] is empty, [aux] is the sorted version 
+  of the input list [l].
+  
+  In a typical insertion sort, you can do binary search on [aux] list and 
+  insert, leading to O(n log(n)) running time. We will just do a linear search
+  through [aux] to find the correct position.
+
+  We will use the comparison function [compare] that you have seen in the
+  assignment. *)
+
+Require Import OrdersFacts.
+
+Check compare.
+Print comparison.
+
+(* In order to prove facts, you will need the definitions from the following. *)
+
+Include (OrderedTypeFacts MidtermSig).
+Include (OrderedTypeTest MidtermSig).
+
+(* Print OrderedTypeFacts. *)
+(* Print OrderedTypeTest. *)
+
+(* FYI, our solution only uses the following three facts, but you may use other 
+   facts. *)
+
+Check compare_gt_iff.
+Check compare_lt_iff.
+Check compare_eq_iff.
+
+(* You will need to define a function [sort] that returns a sorted version 
+   of the input list based on the insertion sorting algorithm above: *)
+  
+Definition sort (l : list t) : list t := l. 
+(* Remove [l] and fill in correct defintion. *)
+(* 5 points *)
+
+(* In order to do the proof, we will define an inductive type called [sorted] 
+   that captures that 
+  
+    (1) An empty list is sorted.
+    (2) A singleton list is sorted.
+    (3) Given a list [l = x::y::t], in order for [l] to be sorted, it better 
+        be the case that [lt x y \/ eq x y] and [sorted (y::t)].
+  
+   Check the definition of [lt] and [eq] below:
+*)
+
+Check lt.
+Check eq.
+
+Inductive sorted : list t -> Prop := . (* FILL IN *)
+(* 5 points *)
+
+(* Prove the following theorem: the result of the [sort] function 
+   returns a [sorted] list. *)
+
+Theorem sort_ok : forall l, sorted (sort l).
+(* 10 points *)
+Proof.
+Abort.
+
+(* Of course, one also needs to prove that the sorted list is a permutation of 
+   the original list. For this, we need to talk about list membership. In Coq, 
+   we use `In` construct to describe list membership. For example, *)
+
+Theorem in_list : In 3 [1;2;3].
+Proof.
+  simplify; equality.
+Qed.
+
+Theorem not_in_list : In 4 [1;2;3] -> False.
+Proof.
+  simplify; equality.
+Qed.
+
+(* Now to the theorem *)
+Theorem sort_is_permutation : forall l e, In e l -> In e (sort l).
+(* 20 points *)
+Proof.
+Abort.
+
+(* You may need some intermediate lemmas based on the intermediate functions 
+   that you may have written down. *)
