assignments/midterm/MidtermSig.v
@@ -1,0 +1,4 @@
+Require Import Frap Datatypes Orders.
+Export Datatypes Orders.
+
+Include OrderedType.
