assignments/midterm/midterm.fst
@@ -1,0 +1,58 @@
+module Midterm
+
+open FStar.List.Tot
+
+(* In this module, we will describe and prove properties about vector clocks.
+   For more information about vector clocks, see:
+   https://en.wikipedia.org/wiki/Vector_clock.
+
+	 You solution should not contain any [admit()] or equivalent. *)
+
+(* The type of vector clock indexed by length *)
+type t (n:nat) = lst:list nat{n > 0 && length lst = n}
+
+type ordering =
+| Happened_before
+| Happened_after
+| Concurrent
+| Equal
+
+val compare : v1:list nat -> v2:list nat{length v1 = length v2} -> ordering
+let rec compare v1 v2 =
+  match v1, v2 with
+  | [], [] -> Equal
+  | x::xs, y::ys ->
+      if x = y then compare xs ys
+      else if x < y then
+        match compare xs ys with
+        | Equal | Happened_before -> Happened_before
+        | _ -> Concurrent
+      else match compare xs ys with
+           | Equal | Happened_after -> Happened_after
+           | _ -> Concurrent
+
+val hb: n:nat -> v1:t n -> v2:t n -> bool
+let hb n a b = compare a b = Happened_before
+
+val hbeq: n:nat -> v1:t n -> v2:t n -> bool
+let hbeq n a b =
+  match compare a b with
+  | Happened_before | Equal -> true
+  | _ -> false
+
+(* 5 points *)
+val hbeq_reflexive : n:nat -> v:t n -> Lemma (ensures (hbeq n v v))
+let hbeq_reflexive n v = admit ()
+
+(* 10 points *)
+val hbeq_transitive : n:nat -> v1:t n -> v2:t n{hbeq n v1 v2} -> v3:t n{hbeq n v2 v3}
+                    -> Lemma (ensures (hbeq n v1 v3))
+let hbeq_transitive n v1 v2 v3 = admit ()
+
+val concurrent : n:nat -> v1:t n -> v2:t n -> bool
+let concurrent n v1 v2 = compare v1 v2 = Concurrent
+
+(* 15 points *)
+val concurrent_commutative : n:nat -> v1:t n -> v2:t n{concurrent n v1 v2}
+                           -> Lemma (ensures (concurrent n v2 v1))
+let concurrent_commutative n v1 v2 = admit ()
